src/program_proof/simplepb/pb_start_proof.v
@@ -1,0 +1,86 @@
+From Perennial.program_proof Require Import grove_prelude.
+From Goose.github_com.mit_pdos.gokv.simplepb Require Export pb.
+From Perennial.program_proof.grove_shared Require Import urpc_proof urpc_spec.
+From Perennial.program_proof.simplepb Require Import pb_definitions pb_applybackup_proof pb_setstate_proof pb_getstate_proof pb_becomeprimary_proof pb_apply_proof pb_makeclerk_proof.
+
+Section pb_start_proof.
+
+Context {pb_record:PBRecord}.
+Notation pbG := (pbG (pb_record:=pb_record)).
+Notation OpType := (pb_OpType pb_record).
+Notation has_op_encoding := (pb_has_op_encoding pb_record).
+Notation has_snap_encoding := (pb_has_snap_encoding pb_record).
+Notation has_op_encoding_injective := (pb_has_op_encoding_injective pb_record).
+Notation compute_reply := (pb_compute_reply pb_record).
+
+Notation wp_Clerk__ApplyAsBackup := (wp_Clerk__ApplyAsBackup (pb_record:=pb_record)).
+Notation wp_Clerk__SetState := (wp_Clerk__SetState (pb_record:=pb_record)).
+Notation wp_Clerk__GetState := (wp_Clerk__GetState (pb_record:=pb_record)).
+Notation wp_Clerk__BecomePrimary := (wp_Clerk__BecomePrimary (pb_record:=pb_record)).
+Notation wp_Clerk__Apply := (wp_Clerk__Apply (pb_record:=pb_record)).
+
+Context `{!heapGS Σ}.
+Context `{!pbG Σ}.
+
+Implicit Type (own_StateMachine: u64 → list OpType → bool → (u64 → list OpType → bool → iProp Σ) → iProp Σ).
+Lemma wp_MakeServer sm_ptr own_StateMachine (epoch:u64) σ (sealed:bool) (nextIndex:u64) γ γsrv :
+  {{{
+        "Hstate" ∷ own_StateMachine epoch σ.*1 sealed (own_Server_ghost γ γsrv) ∗
+        "#His_sm" ∷ is_StateMachine sm_ptr own_StateMachine (own_Server_ghost γ γsrv) ∗
+        "#Hsys_inv" ∷ sys_inv γ ∗
+        "%HnextIndex" ∷ ⌜int.nat nextIndex = length σ⌝ ∗
+
+        (* FIXME: the pb user shouldn't need to know about these. Wrap this up in something *)
+        (* It should be possible to get rid of these from *)
+        "#Hs_acc_lb" ∷ is_accepted_lb γsrv epoch σ ∗
+        "#Hs_prop_lb" ∷ is_proposal_lb γ epoch σ ∗
+        "#Hs_prop_facts" ∷ is_proposal_facts γ epoch σ ∗
+        "#Hs_epoch_lb" ∷ is_epoch_lb γsrv epoch
+  }}}
+    pb.MakeServer #sm_ptr #nextIndex #epoch #sealed
+  {{{
+        s, RET #s; is_Server s γ γsrv
+  }}}
+.
+Proof.
+  iIntros (Φ) "Hpre HΦ".
+  iNamed "Hpre".
+  wp_call.
+  Opaque zero_val.
+  wp_apply (wp_allocStruct).
+  { Transparent slice.T. Transparent zero_val. repeat econstructor. Opaque slice.T. Opaque zero_val. }
+  iIntros (s) "Hs".
+  iDestruct (struct_fields_split with "Hs") as "HH".
+  iNamed "HH".
+  simpl.
+  wp_pures.
+  wp_apply (wp_new_free_lock).
+  iIntros (mu) "HmuInv".
+  wp_storeField.
+  wp_storeField.
+  wp_storeField.
+  wp_storeField.
+  wp_storeField.
+  wp_storeField.
+  iApply "HΦ".
+  iMod (readonly_alloc_1 with "mu") as "#Hmu".
+  iExists _, _.
+  iFrame "Hmu Hsys_inv".
+  iMod (alloc_lock with "HmuInv [-]") as "$"; last done.
+
+  (* now just need to establish lock invariant *)
+  iNext.
+  iExists _,_,_,_,_,_,_.
+  iFrame "∗".
+  iSplitL "clerks".
+  {
+    iApply to_named.
+    instantiate (1:=Slice.nil).
+    iExact "clerks".
+  }
+  iSplitR; first iExact "His_sm".
+  iFrame "#".
+  done.
+Qed.
+
+End pb_start_proof.
